---
tags: mathematics, abstract_algebra
---

# Definition

- $a \equiv a'\ (\text{mod}\ n) \land b \equiv b'\ (\text{mod}\ n) \implies$
	- $a + b \equiv a' + b'\ (\text{mod}\ n) \land a - b \equiv a' - b'\ (\text{mod}\ n)$
	- $ab \equiv a'b'\ (\text{mod}\ n)$
- $a \equiv b\ (\text{mod}\ n) \land b \equiv c\ (\text{mod}\ n) \implies a \equiv c\ (\text{mod}\ n)$ ([[Transitive]])
- $a \equiv b\ (\text{mod}\ n) \land c \in \mathbb{Z} \implies ca \equiv cb\ (\text{mod}\ n)$
- $a \equiv b\ (\text{mod}\ n) \land k \in \mathbb{N} \implies a^k \equiv b^k\ (\text{mod}\ n)$