---
tags: mathematics, real_analysis
---

# Definition

> [!abstract] Theorem 1 (Infinity Case)
> Let $a_n, b_n$ be [[Sequence]] and $b_n$ is strictly [[Monotone Sequence]] and [[Divergent Sequence]]. Then
> $$
> \begin{align}
> \lim_{n \rightarrow \infty} \frac{a_{n+1} - a_n}{b_{n+1} - b_n} = L \implies \lim_{n \rightarrow \infty} \frac{a_n}{b_n} = L
> \end{align}
> $$

> [!abstract] Theorem 2 (Zero Case)
> Let $a_n, b_n$ be [[Sequence]] with $a_n \rightarrow 0, b_n \rightarrow 0$, and $b_n$ is strictly [[Decreasing Sequence]]. Then
> $$
> \begin{align}
> \lim_{n \rightarrow \infty} \frac{a_{n+1} - a_n}{b_{n+1} - b_n} = L \implies \lim_{n \rightarrow \infty} \frac{a_n}{b_n} = L
> \end{align}
> $$

[[L'Hospital's Rule]], but for [[Sequence]].